\documentclass{article}
\usepackage[T1]{fontenc}
\usepackage{pgf,tikz,tikzscale} 
\usepackage{amssymb}
\usepackage{tcolorbox}
\usepackage{xcolor}
\usepackage[utf8]{inputenc}
\usepackage[english]{babel}
\usepackage{multicol}
\usepackage{enumerate}	
\usepackage{graphicx,lipsum,pgfplots} 
\usepackage{amsmath, amsthm}                 
\usepackage[top=1in,bottom=1in, left=.5in, right=.5in] {geometry}  
\usepackage{fancyhdr}       

\newcommand{\Var}{\operatorname{Var}} %% \Var{X}
\newcommand{\Cov}{\operatorname{Cov}}

\newcommand{\var}{\operatorname{var}} %% \Var{X}
\newcommand{\cov}{\operatorname{cov}}

\pagestyle{fancy}              
\lhead{Stat 5930 \newline Homework Chapter 3 \#7}   
\rhead{Warren Keil}






\begin{document}
\setlength{\parindent}{0cm}   %%%%%%%% KEEP THIS  for block style para. 



%%%%%%%%%%%%%%%%%        1a   %%%%%%%%%%%%%%%%%%%%
\textbf{1.} Show that if \(rank(A) = q\), then
\[
E[RSS_H - RSS] = \sigma^2q + (A\beta)'(A(X'X)^-A')^{-1}(A\beta)
\]


\vspace{5mm}
\textbf{\textsc{Proof.}} First observe that  from section 3.8.1 and using formula 4.3, \(\hat \beta_H= \hat \beta + (X'X)^{-1}A'[A(X'X)^{-1}A']^{-1}(A\hat\beta-c)\) , we find, 
\begin{align*}
RSS_H - RSS &= ||\hat Y - \hat Y_H ||^2 \\
&= (\hat \beta-\hat\beta_H)'X'X(\hat \beta-\hat\beta_H). \\
&= (\hat\beta - \hat \beta + (X'X)^{-1}A'[A(X'X)^{-1}A']^{-1}(A\hat\beta-c))'X'X(\hat\beta - \hat \beta + (X'X)^{-1}A'[A(X'X)^{-1}A']^{-1}(A\hat\beta-c))\\
&= ((X'X)^{-1}A'[A(X'X)^{-1}A']^{-1}(A\hat\beta-c))'X'X((X'X)^{-1}A'[A(X'X)^{-1}A']^{-1}(A\hat\beta-c))\\
&= (A\hat\beta-c)' [A(X'X)^{-1}A']^{-1} A(X'X)^{-1} X'X((X'X)^{-1}A'[A(X'X)^{-1}A']^{-1}(A\hat\beta-c))\\
&= (A\hat\beta-c)' [A(X'X)^{-1}A']^{-1} A((X'X)^{-1}A'[A(X'X)^{-1}A']^{-1}(A\hat\beta-c))\\
&= (A\hat\beta-c)' [A(X'X)^{-1}A']^{-1}(A\hat\beta-c)).\\
\end{align*}

Next, from section 2.2 in the text, we know that \(\hat\beta \sim N_p(\beta,\sigma^2(X'X)^{-1}) \) and thus,  \(A\hat\beta \sim N_p(A\beta,\sigma^2A(X'X)^{-1}A') \). Then if we let \(Z= A\hat\beta-c\) and \( B = A(X'X)^{-1}A' \) , we get that 
\[
E[Z] = A\beta -c, \hspace{15mm} \Var[Z] =\Var[A\hat\beta] = \sigma^2B.
\]
Now we refer to theorem 1.5 which shows the form of the expected value of quadratics forms, 
\begin{align*}
E[RSS_H - RSS] &= E[(A\hat\beta-c)' [A(X'X)^{-1}A']^{-1}(A\hat\beta-c)) \\
&= E[Z'B^{-1}Z]  \\
&= tr(\sigma^2B^{-1}B) + (A\beta-c)'B^{-1}(A\beta-c)\\
&= tr(\sigma^2I_q) + (A\beta-c)'B^{-1}(A\beta-c) \\
&= \sigma^2q + (A\beta-c)'B^{-1}(A\beta-c) \\
&=  \sigma^2q + (A\beta-c)'[A(X'X)^{-1}A']^{-1}(A\beta-c) \\
\end{align*}

\begin{flushright}
\(\qed\)\end{flushright}







\newpage
\textbf{2.} Let
\begin{align*}
Y_1 &= \theta_1 + \theta_2 + \epsilon_1 \\
Y_2 &= 2\theta_2 + \epsilon_2 \\
Y_3 &= -\theta_1 + \theta_2 + \epsilon_3
\end{align*}
where the \(\epsilon_i\) are iid \(N(0,\sigma^2) \). Derive the F statistic for testing the hypothesis \(H:\theta_1=2\theta_2\). 

\vspace{5mm}
\textbf{\textsc{Solution.}} 

\begin{flushright}
\(\qed\)\end{flushright}

\newpage
\textbf{3.} Given the two regression lines
\[
Y_{ki} = \beta_k+\epsilon_{ki}, \hspace{3cm} k=1,2,\ldots, n.
\]
show that the Fstatistic for testing \(H: \beta_1=\beta_2\) can be written as 
\[
F = \frac{ (\hat \beta_1 - \hat \beta_2 )^2 }{(2S^2(\sum_i x_i^2)^{-1}}. 
\]
Obtain \(RSS\) and \(RSS_H\) and verify that \(RSS_H - RSS= \sum_i x_i^2(\hat \beta_1 - \hat \beta_2)^2 /2\) 

\vspace{5mm}
\textbf{\textsc{Solution.}} 

\begin{flushright}
\(\qed\)\end{flushright}

\newpage
\textbf{4.} Prove that \((RSS_H-RSS)/\sigma^2 \) has a non-central chi-squared distribution with non-centrality parameter,
 \[\lambda = \mu'(P_\Omega~-P_\omega)\mu/2\sigma^2. \]


\vspace{5mm}
\textbf{\textsc{Solution.}} 

\begin{flushright}
\(\qed\)\end{flushright}

\end{document} 






























